\section{A Guide to the Derivation of Equations \eqref{eq:HKM_HRd}--\eqref{eq:NT_M}} \label{sec:guide_for_dir_eq}

% \begin{equation}
%     \everymath{\displaystyle}
%     \renewcommand{\arraystretch}{2.5}
%     \begin{array}{rl}
%        & \sum_{p=1}^P \mathcal{A}^p(\Delta x^p) = R_{prim} \\
%        \Leftrightarrow 
%        & \sum_{p = u} \mathcal{A}^p(\Delta x^p) + \sum_{p \neq u} \mathcal{A}^p(\Delta x^p) = R_{prim} \\
%        \Leftrightarrow 
%        & \sum_{p = u} \mathcal{A}^p((\mathcal{E}^p)^{-1}R_{comp}^p - \mathcal{H}^p(R_{dual}^p - \mathcal{A}^p(\Delta y))) + \sum_{p \neq u} \mathcal{A}^p(\Delta x^p) = R_{prim} \\
%        \Leftrightarrow 
%        & \sum_{p = u} \mathcal{A}^p\mathcal{H}^p(\mathcal{A}^p)^T\Delta y = h :=  R_{prim} - \sum_{p = u} \mathcal{A}^p((\mathcal{E}^p)^{-1}R_{comp}^p - \mathcal{H}^p R_{dual}^p) - \sum_{p \neq u} \mathcal{A}^p(\Delta x^p)
%     \end{array}
% \end{equation}

% \begin{align*}
% a>0 \quad \text{and} \quad c>0 
% & \Rightarrow (\Delta x^p)_0 > \|\Delta \bar{x}^p\| \quad \text{and} \quad (x^p)_0 > \|\bar{x}^p\| \\
% & \Rightarrow (\Delta x^p)_0 (x^p)_0 > \|\Delta \bar{x}^p\|\|\bar{x}^p\| \geq (\Delta \bar{x}^p)^T \bar{x}^p \\
% & \Rightarrow b = (\Delta x^p)_0 (x^p)_0 - (\Delta \bar{x}^p)^T \bar{x}^p > 0
% \end{align*}

In the case of $\mathbb{K}^p=\mathbb{S}_+^{n_p}$, the derivation for the HKM direction is straightforward by noting that $G^p=(z^p)^\frac{1}{2}$ and $\mathcal{E}\Delta x = ((z^p)^\frac{1}{2}\Delta x^p)\circ ((z^p)^{-\frac{1}{2}}z^p)=(z^p)^\frac{1}{2} \Delta x^p (z^p)^\frac{1}{2}$.
For the NT direction, the derivation is non-trivial and can be found in \cite{todd1998}.
In the case of $\mathbb{K}^p=\mathbb{Q}^{n_p}$, for $f\in \mathbb{R}^{n^p}$, %define the linear operator $Arw: \mathbb{R}^{n_p} \rightarrow \mathbb{R}^{n\times n}$ as
\begin{equation}
    \operatorname{Arw}(f) = 
    \left(
    \begin{array}{cc}
        f_0 & \bar{f}^T \\
        \bar{f} & f_0 I
    \end{array}
    \right)
\end{equation}
then $x^p \circ z^p = \operatorname{Arw}(x^p)z^p$ holds, so
\begin{align*}
    (\mathcal{E}^p)^{-1}R^p_{comp} &= G^p \cdot \operatorname{Arw}(G^p x^p)^{-1} \cdot R^p_{comp}\\
    \mathcal{H}^p R^p_{dual} &= G^p \cdot \operatorname{Arw}(G^p x^p)^{-1} \cdot \operatorname{Arw}\big((G^p)^{-1} z^p\big) \cdot(G^p)^{-1} \cdot R^p_{dual}\\
    \mathcal{A}^p\mathcal{H}^p(\mathcal{A}^p)^T &= A^p \cdot G^p \cdot \operatorname{Arw}(G^p x^p)^{-1} \cdot \operatorname{Arw}\big((G^p)^{-1} z^p\big) \cdot(G^p)^{-1} \cdot (A^p)^T
\end{align*}
can be generally described. Furthermore,
\begin{equation*}
    \operatorname{Arw}(f)^{-1} = \frac{1}{\gamma(f)^2} \left(\begin{array}{cc}
        f_0 & -\bar{f}^T \\
        -\bar{f} & \frac{1}{f_0}(\gamma(f)^2 I + \bar{f}\bar{f}^T)
    \end{array}\right),
    \qquad
    (G^p)^{-1} = \frac{1}{\omega^p} \begin{pmatrix}
        t^p_0 & -(\bar{t}^p)^T \\
        -\bar{t}^p & I+\frac{1}{1 + t^p_0} \bar{t}^p(\bar{t}^p)^T
    \end{pmatrix}
\end{equation*}
holds (note that $\gamma(t)=1$ is assumed), which can be used to derive equations \eqref{eq:HKM_HRd}--\eqref{eq:NT_M}.
In the case of $\mathcal{K}^p=\mathbb{R}^{n_p}_+$, the derivation is straightforward by noting that $\mathcal{E}^p \Delta x^p = \operatorname{diag}(z^p) \Delta x^p$.